theories/FRACTRAN/FRACTRAN_dec.v
@@ -1,0 +1,30 @@
+(*
+  Author(s):
+    Hizbullah Abdul Aziz Jabbar (1)
+    Andrej Dudenhefner (2)
+    Dominique Larchey-Wendling (3)
+  Affiliation(s):
+    (1) Saarland University, Saarbrücken, Germany
+    (2) TU Dortmund University, Dortmund, Germany
+    (3) LORIA -- CNRS
+*)
+
+(*
+  Decidability Results(s):
+    Decidability of Reversible FRACTRAN Halting (Halt_REV_FRACTRAN_dec)
+*)
+
+Require Import Undecidability.Synthetic.Definitions.
+
+Require Import Undecidability.FRACTRAN.FRACTRAN.
+From Undecidability.FRACTRAN.Deciders Require
+  Halt_REV_FRACTRAN_dec.
+
+(* Decidability of Reversible FRACTRAN Halting *)
+Theorem Halt_REV_FRACTRAN_dec : decidable Halt_REV_FRACTRAN.
+Proof.
+  exists Halt_REV_FRACTRAN_dec.decide.
+  exact Halt_REV_FRACTRAN_dec.decide_spec.
+Qed.
+
+Check Halt_REV_FRACTRAN_dec.
